Verifying interop memcpy

src/arch/x64/interop/Memcpy.fst
@@ -28,7 +28,6 @@ module BS = X64.Bytes_Semantics_s
 open Vale_memcpy
 
 #set-options "--initial_fuel 5 --max_fuel 5 --initial_ifuel 2 --max_ifuel 2"
-
 let create_initial_state w dst src stack_b (h0:HS.mem{pre_cond h0 dst src /\ B.length stack_b == 24 /\ live h0 stack_b /\ buf_disjoint_from stack_b [dst;src]}) : GTot TS.traceState =
   let taint_func (x:b8) : GTot taint =
     if StrongExcludedMiddle.strong_excluded_middle (x == dst) then Secret else
@@ -57,22 +56,65 @@ let create_initial_state w dst src stack_b (h0:HS.mem{pre_cond h0 dst src /\ B.l
   let s0:X64.Memory_i_s.state = {ME.state = s_b; ME.mem = mem} in
   {TS.state = s0; TS.trace = []; TS.memTaint = create_valid_memtaint mem buffers taint_func}
 
+let create_initial_vale_state w dst src stack_b (h0:HS.mem{pre_cond h0 dst src /\ B.length stack_b == 24 /\ live h0 stack_b /\ buf_disjoint_from stack_b [dst;src]}) : GTot va_state =
+  let taint_func (x:b8) : GTot taint =
+    if StrongExcludedMiddle.strong_excluded_middle (x == dst) then Secret else
+    if StrongExcludedMiddle.strong_excluded_middle (x == src) then Secret else
+    Public in
+  let buffers = stack_b::dst::src::[] in
+  let (mem:mem) = {addrs = addrs; ptrs = buffers; hs = h0} in
+  let addr_dst = addrs dst in
+  let addr_src = addrs src in
+  let addr_stack:nat64 = addrs stack_b + 0 in
+  let regs = if w then (
+    fun r -> begin match r with
+      | Rsp -> addr_stack
+      | Rcx -> addr_dst
+      | Rdx -> addr_src
+      | _ -> init_regs r end)
+  else (
+    fun r -> begin match r with
+      | Rsp -> addr_stack
+      | Rdi -> addr_dst
+      | Rsi -> addr_src
+      | _ -> init_regs r end)
+  in
+  let xmms = init_xmms in
+  {ok = true; regs = regs; xmms = xmms; flags = 0; mem = mem; memTaint =    create_valid_memtaint mem buffers taint_func}
+
+let create_lemma w dst src stack_b (h0:HS.mem{pre_cond h0 dst src /\ B.length stack_b == 24 /\ live h0 stack_b /\ buf_disjoint_from stack_b [dst;src]}) : Lemma
+  (state_of_S (create_initial_state w dst src stack_b h0) == create_initial_vale_state w dst src stack_b h0) =
+    let s_init = create_initial_state w dst src stack_b h0 in
+    let s0 = state_of_S s_init in
+    let s1 = create_initial_vale_state w dst src stack_b h0 in
+    assert (FunctionalExtensionality.feq s1.regs (regs' s_init.TS.state));
+    assert (FunctionalExtensionality.feq s1.xmms (xmms' s_init.TS.state));
+    lemma_of_ok s_init;
+    lemma_of_regs s_init;
+    lemma_of_flags s_init;
+    lemma_of_xmms s_init;    
+    lemma_of_mem s_init;
+    lemma_of_memTaint s_init;
+    ()
+
 let implies_pre (w:bool) (h0:HS.mem) (dst:s8) (src:s8)  (stack_b:b8) : Lemma
   (requires pre_cond h0 dst src /\ B.length stack_b == 24 /\ live h0 stack_b /\ buf_disjoint_from stack_b [dst;src])
   (ensures (
   B.length stack_b == 24 /\ live h0 stack_b /\ buf_disjoint_from stack_b [dst;src] /\ (
-  let s0 = state_of_S (create_initial_state w dst src stack_b h0) in
+  let s0 = create_initial_vale_state w dst src stack_b h0 in
   length_t_eq (TBase TUInt64) stack_b;
   length_t_eq (TBase TUInt64) dst;
   length_t_eq (TBase TUInt64) src;
-  va_pre (va_code_memcpy w) s0 w stack_b dst src))) =
-  admit()
-  // length_t_eq (TBase TUInt64) stack_b;
-  // length_t_eq (TBase TUInt64) dst;
-  // length_t_eq (TBase TUInt64) src;
-  // assert(B.disjoint stack_b dst);
-  // assert(B.disjoint stack_b src);
-  // ()
+  va_pre (va_code_memcpy w) s0 w stack_b dst src ))) =
+  length_t_eq (TBase TUInt64) stack_b;
+  length_t_eq (TBase TUInt64) dst;
+  length_t_eq (TBase TUInt64) src;
+  assert(B.disjoint stack_b dst);
+  assert(B.disjoint stack_b src);
+  ()
+
+let seq_nat64_to_seq_U64 (b:Seq.seq nat64) : (Seq.seq UInt64.t) =
+  Seq.init (Seq.length b) (fun (i:nat { i < Seq.length b }) -> UInt64.uint_to_t (Seq.index b i))
 
 let implies_post (w:bool) (va_s0:va_state) (va_sM:va_state) (va_fM:va_fuel) (dst:s8) (src:s8)  (stack_b:b8) : Lemma
   (requires pre_cond va_s0.mem.hs dst src /\ B.length stack_b == 24 /\ live va_s0.mem.hs stack_b /\ buf_disjoint_from stack_b [dst;src] /\
@@ -81,13 +123,19 @@ let implies_post (w:bool) (va_s0:va_state) (va_sM:va_state) (va_fM:va_fuel) (dst
   length_t_eq (TBase TUInt64) stack_b;
   length_t_eq (TBase TUInt64) dst;
   length_t_eq (TBase TUInt64) src;
+  let dst_b = BV.mk_buffer_view dst Views.view64 in
+  let src_b = BV.mk_buffer_view src Views.view64 in
+  // assert (buffer64_read dst 0 (va_get_mem va_sM) == UInt64.v (Seq.index (BV.as_seq va_sM.mem.hs dst_b) 0);
+  let t = TBase TUInt64 in
+  assert (Seq.equal (seq_nat64_to_seq_U64 (buffer_as_seq #t (va_get_mem va_sM) src)) (BV.as_seq va_sM.mem.hs src_b));  
+  assert (Seq.equal (seq_nat64_to_seq_U64 (buffer_as_seq #t (va_get_mem va_sM) dst)) (BV.as_seq va_sM.mem.hs dst_b));  
   ()
 
 val lemma_ghost_memcpy:  w:bool -> dst:s8 -> src:s8 ->  stack_b:b8 -> (h0:HS.mem{pre_cond h0 dst src /\ B.length stack_b == 24 /\ live h0 stack_b /\ buf_disjoint_from stack_b [dst;src]}) ->
   Ghost (TS.traceState * nat * HS.mem)
     (requires True)
     (ensures (fun (s1, f1, h1) ->
-      (let s0:TS.traceState = create_initial_state w dst src stack_b h0 in
+      (let s0 = create_initial_state w dst src stack_b h0 in
        Some s1 == TS.taint_eval_code (va_code_memcpy w) f1 s0 /\
        s1.TS.state.ME.state.BS.mem == Interop.down_mem h1 addrs [stack_b;dst;src] /\
        post_cond h0 h1 dst src /\
@@ -96,20 +144,25 @@ val lemma_ghost_memcpy:  w:bool -> dst:s8 -> src:s8 ->  stack_b:b8 -> (h0:HS.mem
     )
 
 
-let lemma_ghost_memcpy w dst src stack_b h0 =
+let lemma_ghost_memcpy w dst src stack_b h0 = admit() (*
   length_t_eq (TBase TUInt64) stack_b;
   length_t_eq (TBase TUInt64) dst;
   length_t_eq (TBase TUInt64) src;
   implies_pre w h0 dst src stack_b ;
   let s0 = create_initial_state w dst src stack_b h0 in
+  create_lemma w dst src stack_b h0;
   let s_v, f_v = va_lemma_memcpy (va_code_memcpy w) (state_of_S s0) w stack_b dst src in  
   implies_post w (state_of_S s0) s_v f_v dst src stack_b;
   Some?.v (TS.taint_eval_code (va_code_memcpy w) f_v s0), f_v, s_v.mem.hs
+*)
 
 let memcpy dst src  =
   push_frame();
   let (stack_b:b8) = B.alloca (UInt8.uint_to_t 0) (UInt32.uint_to_t 24) in
   st_put 
   (fun h -> pre_cond h dst src /\ B.length stack_b == 24 /\ live h stack_b /\ buf_disjoint_from stack_b [dst;src]) 
-  (fun h -> let _, _, h1 = lemma_ghost_memcpy win dst src stack_b h in h1);
+  (fun h -> let _, _, h1 = 
+    if win then lemma_ghost_memcpy true dst src stack_b h
+    else lemma_ghost_memcpy false dst src stack_b h
+  in h1);
   pop_frame()
